theories/RTac/Solve.v
@@ -1,5 +1,6 @@
 Require Import ExtLib.Tactics.
 Require Import MirrorCore.RTac.Core.
+Require Import MirrorCore.RTac.IsSolved.
 
 Require Import MirrorCore.Util.Forwardy.
 
@@ -16,10 +17,39 @@ Section parameterized.
 
   Definition SOLVE (tac : rtac typ expr) : rtac typ expr :=
     fun tus tvs nus nvs ctx s g =>
-      match tac tus tvs nus nvs ctx s g with
-        | Solved s => Solved s
-        | _ => Fail
+      match is_solved (tac tus tvs nus nvs ctx s g) with
+      | Some s => Solved s
+      | _ => Fail
       end.
+
+  Lemma Proper_rtac_spec_impl : forall
+      (ctx : Ctx typ expr) (s : ctx_subst ctx),
+      Morphisms.Proper
+        (Morphisms.respectful (fun x y => GoalImplies (s,x) (s,y))
+                              (Morphisms.respectful (Basics.flip (ImplResult (c:=ctx))) (Basics.flip Basics.impl))) 
+        (rtac_spec s).
+  Proof.
+    do 3 red. simpl.
+    intros.
+    red. intro.
+    eapply rtac_spec_rtac_spec_modular; try reflexivity.
+    eapply rtac_spec_rtac_spec_modular in H1; try reflexivity.
+    unfold rtac_spec_modular in *. revert H1.
+    inversion H0; clear H0; auto.
+    simpl.
+    clear H1 H2.
+    destruct x1; destruct y1; simpl in *.
+    intros; forward_reason.
+    split; auto.
+    split; auto.
+    forward. forward_reason.
+    split.
+    { etransitivity; eauto. }
+    { intros.
+      repeat progress (gather_facts;
+                       eapply pctxD_SubstMorphism; [ | | eassumption | ]; eauto).
+      eapply Pure_pctxD; eauto. }
+  Qed.
 
   Theorem SOLVE_sound
   : forall tac, rtac_sound tac -> rtac_sound (SOLVE tac).
@@ -27,10 +57,13 @@ Section parameterized.
     unfold SOLVE, rtac_sound.
     intros.
     specialize (H ctx s g).
-    subst; destruct (tac (getUVars ctx) (getVars ctx)
-           (length (getUVars ctx)) (length (getVars ctx)) ctx s g); auto.
-    specialize (H _ eq_refl).
-    eapply rtac_spec_Fail.
+    destruct (is_solved (tac (getUVars ctx) (getVars ctx) (length (getUVars ctx))
+              (length (getVars ctx)) ctx s g)) eqn:?; subst; try apply rtac_spec_Fail.
+    eapply is_solved_sound in Heqo.
+    eapply Proper_rtac_spec_impl.
+    { reflexivity. }
+    { eapply Heqo. }
+    { eapply H. reflexivity. }
   Qed.
 
   Fixpoint SOLVES (tacs : list (rtac typ expr)) : rtac typ expr :=
@@ -39,8 +72,8 @@ Section parameterized.
     | tac :: tacs =>
       let rec := SOLVES tacs in
       fun tus tvs nus nvs ctx s g =>
-        match tac tus tvs nus nvs ctx s g with
-        | Solved s => Solved s
+        match is_solved (tac tus tvs nus nvs ctx s g) with
+        | Some s => Solved s
         | _ => rec tus tvs nus nvs ctx s g
         end
     end.
@@ -52,10 +85,13 @@ Section parameterized.
     { red. intros; subst. eapply rtac_spec_Fail. }
     { red.
       intros.
-      specialize (H ctx s g _ eq_refl).
-      destruct (x (getUVars ctx) (getVars ctx)
-                  (length (getUVars ctx)) (length (getVars ctx)) ctx s g); auto.
-      subst; auto. }
+      destruct (is_solved (x (getUVars ctx) (getVars ctx) (length (getUVars ctx))
+                             (length (getVars ctx)) ctx s g)) eqn:?; subst; eauto.
+      eapply is_solved_sound in Heqo.
+      eapply Proper_rtac_spec_impl.
+      { reflexivity. }
+      { eapply Heqo. }
+      { eapply H. reflexivity. } }
   Qed.
 
 End parameterized.
